Session.v
@@ -1,8 +1,4 @@
-Require Export SfLib.
-Require Export CpdtTactics.
 Require Export Crypto.
-
-Module session.
 
 Inductive protoType : Type :=
 | Send : type -> protoType -> protoType
@@ -11,9 +7,6 @@ Inductive protoType : Type :=
 | Offer : protoType -> protoType -> protoType  
 | Eps : type -> protoType.
 
-
-Definition t1 := Send (Basic) (Eps Basic). Check t1.
-  
 Inductive protoExp : type -> protoType -> Type :=
 | SendC {t:type} {T:type} {p':protoType}  : (message t) -> (protoExp T p')
     -> protoExp T (Send t p')
@@ -53,83 +46,15 @@ Notation "'offer'" := OfferC.
 Notation "'choice'" := ChoiceC.
 
 Definition EpsC := ReturnC (basic 0).
-Definition proto1 := SendC (basic 1) EpsC.
-Check proto1.
-
-Definition unwrapBasic (m:message Basic) : nat :=
-  match m with
-  | basic n => n
-  | _ => 0
-  end.
-
-
-Definition enc1 := encrypt (basic 42) (public 1). Check enc1.
-Definition enc2 := encrypt enc1 (public 2).
-Eval compute in decryptM enc1 (private 1).
-Eval compute in decryptM enc1 (private 0).
-Eval compute in decryptM enc2 (private 2).
-Eval compute in decryptM (decryptM enc2 (private 2)) (private 1).
-
-Definition getP1Type (t:type):type :=
-  match t with
-  | Pair t1 t2 => t1
-  | _ => t
-  end.
-
-Definition getP2Type (t:type):type :=
-  match t with
-  | Pair t1 t2 => t2
-  | _ => t
-  end.
-
-Definition pairFst{t1 t2: type} (m:message (Pair t1 t2)) : message t1 :=
-  match m in message t' return message (getP1Type t') with 
-  | pair _ _ m1 _ => m1
-  | bad _ => bad _ (*(getP1Type tb1) *)
-  | _ => bad _                
-  end.
-
-Definition pair1 := pair (basic 1) (basic 2).
-Eval compute in pairFst pair1.
-Definition pair1' := pair (bad Basic) (basic 2).
-Eval compute in pairFst pair1'.
-Definition pair1'' := pair  (basic 1) (bad Basic).
-Eval compute in pairFst pair1''.
-
-Definition pairSnd{t1 t2: type} (m:message (Pair t1 t2)) : message t2 :=
-  match m in message t' return message (getP2Type t') with
-  | pair _ _ _ m2 => m2
-  | bad _ => bad _ (*(getP1Type tb1) *)
-  | _ => bad _                
-  end.
-
-Definition pair2 := pair (basic 1) (basic 2).
-Eval compute in pairSnd pair2.
-Definition pair2' := pair (basic 1) (bad Basic).
-Eval compute in pairSnd pair2'.
-
-(*Fixpoint protoTypeLength (t:protoType) : nat :=
-  match t with
-  | Send _ t' => 1 + (protoTypeLength t')
-  | Receive _ t' => 1 + (protoTypeLength t')
-  | Choice p1 p2 => 1 + protoTypeLength p1
-  | Offer p1 p2 => 1 + protoTypeLength p1
-  | Eps _ => 1                               
-  end. *)
 
 Fixpoint protoExpLength {T:type} {pt:protoType} (p: protoExp T pt) : nat :=
   match p with
-  | SendC _ _ _ _ p' => 1 + (protoExpLength p')
-  | ReceiveC t _ _ f => 1 + (protoExpLength (f (bad t)))
-  | ChoiceC b _ _ _ _ p' p'' => if b then (protoExpLength p')
-                               else (protoExpLength p'')
-  | OfferC _ _ _ _ p' p'' => max (protoExpLength p') (protoExpLength p'')
-  | ReturnC _ _ => 1
-  end.                                                                                   
-
-Definition protoLength {t:protoType} {T:type} (p1:protoExp T t) : nat := (*protoTypeLength t*) protoExpLength p1.
-
-(*Eval compute in protoTypeLength (Send Basic (Eps Basic)). *)
+  | SendC  _ p' => 1 + (protoExpLength p')
+  | ReceiveC f => 1 + (protoExpLength (f (bad _)))
+  | ChoiceC b p' p'' =>  max (protoExpLength p') (protoExpLength p'')
+  | OfferC  p' p'' => max (protoExpLength p') (protoExpLength p'')
+  | ReturnC _ => 1
+  end.                                                               
 
 Fixpoint DualT (t t':protoType) : Prop :=
   match t with
@@ -169,22 +94,23 @@ Fixpoint DualT (t t':protoType) : Prop :=
 Fixpoint DualT_dec (t t':protoType) : {DualT t t'} + {~ DualT t t'}.
 Proof. 
   destruct t; destruct t';
+
   (* Eliminate all un-interesting cases *)
   try (right; unfold not; intros; inversion H; contradiction);
 
   (* For the Send/Receive, Receive/Send cases *)
   try (
-  destruct (eq_type_dec t t2); destruct (DualT_dec t0 t');
+  destruct (eq_type_dec t t1); destruct (DualT_dec t0 t');
   try (right; unfold not; intros; inversion H; contradiction);
   try (left; split; assumption)
   );
 
   (* For the Choice/Offer, Offer/Choice cases *)
   try (
-  destruct (DualT_dec t2 t'1); destruct (DualT_dec t3 t'2);
+  destruct (DualT_dec t1 t'1); destruct (DualT_dec t2 t'2);
   try (right; unfold not; intros; inversion H; contradiction);
   try( left; split; assumption)
-    ).
+    );
 
   (* Eps/Eps case *)
   left. simpl. trivial.
@@ -193,206 +119,106 @@ Defined.
 
 Definition Dual {t t':protoType} {T T':type} (p1:protoExp T t) (p2:protoExp T' t') : Prop := DualT t t'.        
 
-Fixpoint runProto'' {t t':protoType} {T T':type} (p1:protoExp T t) (p2:protoExp T' t')  (*(l: nat) *)
+Fixpoint runProto' {t t':protoType} {T T':type} (p1:protoExp T t) (p2:protoExp T' t') 
   : (Dual p1 p2) -> (message T).
 Proof. intros; destruct p1; destruct p2; try inversion H.
 
-       subst. apply (runProto'' _ _ _ _ p1 (p m) (*l*)(*(protoExpLength (p m))*)). assumption.
-       subst. apply (runProto'' _ _ _ _ (p m) p2 ). assumption.
+       subst. apply (runProto' _ _ _ _ p1 (p m) (*l*)(*(protoExpLength (p m))*)). assumption.
+       subst. apply (runProto' _ _ _ _ (p m) p2 ). assumption.
 
        destruct b.
-       apply (runProto'' _ _ _ _ p1_1 p2_1 ). assumption.
-       apply (runProto'' _ _ _ _ p1_2 p2_2 ). assumption.
+       apply (runProto' _ _ _ _ p1_1 p2_1 ). assumption.
+       apply (runProto' _ _ _ _ p1_2 p2_2 ). assumption.
        
        destruct b.
        assert (message R).
-       apply (runProto'' _ _ _ _ p1_1 p2_1 ). assumption. exact (leither _ _ X).
+       apply (runProto' _ _ _ _ p1_1 p2_1 ). assumption. exact (leither _ _ X).
        assert (message S).
-       apply (runProto'' _ _ _ _ p1_2 p2_2 ). assumption. exact (reither _ _ X).
+       apply (runProto' _ _ _ _ p1_2 p2_2 ). assumption. exact (reither _ _ X).
 
-       exact m. Defined.
-
-Definition runProto' {t t':protoType} {T T':type} (p1:protoExp T t) (p2:protoExp T' t')
-  : (Dual p1 p2) -> (message T) := runProto'' p1 p2 (*(1 + (max (protoLength p1) (protoLength p2)))*). Check runProto'.
+       exact m.
+Defined.
 
 Fixpoint DualTSymm {t t':protoType} : DualT t t' -> DualT t' t.
 Proof.
   intros. destruct t; destruct t'; try (inversion H); try (
   split;
   subst; trivial;
-  apply (DualTSymm); assumption). Defined.
+  apply (DualTSymm); assumption).
+Defined.
 
-Hint Resolve DualTSymm.
-
-Lemma DualSymm {t t':protoType} {T T':type} {p1:protoExp T t} {p2:protoExp T' t'} :
-  (Dual p1 p2) -> (Dual p2 p1). intros. unfold Dual in H. apply DualTSymm in H. assumption. Defined.
+Lemma DualSymm {t t':protoType} {T T':type} {p1:protoExp T t} {p2:protoExp T' t'} : (Dual p1 p2) -> (Dual p2 p1).
+Proof.
+  intros. unfold Dual in H. apply DualTSymm in H. assumption.
+Defined.
 
 Lemma notDualSymm {t t':protoType} {T T':type} {p1:protoExp T t} {p2:protoExp T' t'} : (~ Dual p1 p2) -> (~ Dual p2 p1).
 Proof. 
-  intros. unfold not. intros. apply DualTSymm in H0. unfold Dual in H. contradiction. Qed.
+  intros. unfold not. intros. apply DualTSymm in H0. unfold Dual in H. contradiction.
+Defined.
 
-  
 Definition runProto {t t':protoType} {T T':type} (p1:protoExp T t) (p2:protoExp T' t') : (Dual p1 p2) -> (message T * message T') :=
   fun pf =>
     let x := runProto' p1 p2 pf in
     let y := runProto' p2 p1 (DualTSymm pf) in
     (x , y).
 
+Definition nextType{T T':type} {t t':protoType} (p1:protoExp T t) (p2:protoExp T' t') : (Dual p1 p2) -> protoType.
+  intros; destruct p1; destruct p2; try inversion H. exact p'. exact p'. destruct b. exact r. exact s. destruct b. exact r. exact s. exact (Eps t0).
+Defined.
 
-Definition proto3 :=
-  send (basic 42);
-  ReturnC (t:=Basic) (basic 1). Check proto3.
+Definition nextRtype {T T':type} {t t':protoType} (p1:protoExp T t) (p2:protoExp T' t') : (Dual p1 p2) -> type.
+  intros; destruct p1; destruct p2; try inversion H. exact T. exact T. destruct b. exact R. exact S. destruct b. exact R. exact S. exact t0.
+Defined.
 
-Definition proto3' :=
-  x <- receive;
-  ReturnC (t:=Basic) x. Check proto3'.
+Definition runProto'OneStep {t t':protoType} {T T':type} (p1:protoExp T t) (p2:protoExp T' t') (p:Dual p1 p2) : (protoExp (nextRtype p1 p2 p) (nextType p1 p2 p)).
+  destruct p1; destruct p2; try inversion p.
+simpl. destruct p. exact p1.
+simpl. destruct p. subst. exact (p0 m).
+destruct b.
+simpl. destruct p. exact p1_1.
+simpl. destruct p. exact p1_2.
+destruct b.
+simpl. destruct p. exact p1_1.
+simpl. destruct p. exact p1_2.
+simpl. destruct p. exact (ReturnC m0).
+Defined.
 
-Example dual33' : Dual proto3 proto3'. unfold Dual. simpl. auto. Defined.
+Definition runProtoOneStep {t t':protoType} {T T':type} (p1:protoExp T t) (p2:protoExp T' t') (p:Dual p1 p2) : ((protoExp (nextRtype p1 p2 p) (nextType p1 p2 p)) * (protoExp (nextRtype p2 p1 (DualSymm p)) (nextType p2 p1 (DualSymm p)) )) :=
+  let x := (runProto'OneStep p1 p2 p) in
+  let y := (runProto'OneStep p2 p1 (DualTSymm p)) in
+  (x,y).    
 
-Eval compute in (runProto proto3' proto3 dual33').
+Fixpoint runProtoMultiStep' {t t':protoType} {T T':type} (p1:protoExp T t) (p2:protoExp T' t') (n:nat) : (Dual p1 p2) -> (message T * message T').
+  refine
+  ( fun pf => 
+    match n with
+    | O => _
+    | S n' => _
+    end). destruct p1; destruct p2; try inversion pf.
+  exact (bad T, bad T0).
+  exact (bad T, bad T0).
+  destruct b.
+    exact (bad R, bad (Either R0 S0)).
+    exact (bad S, bad (Either R0 S0)).
+  destruct b.
+    exact (bad (Either R S), bad R0).
+    exact (bad (Either R S), bad S0).
+  exact (m, m0).
+  destruct (runProtoOneStep p1 p2 pf);
+  destruct p1; destruct p2; try inversion pf;
+  try
+  (subst; destruct pf; cbv in p;  cbv in p0;  destruct (runProtoMultiStep' _ _ _ _ p p0 n' d); exact (m0, m1)).
+  destruct b.
+  destruct pf. cbv in p. cbv in p0. destruct (runProtoMultiStep' _ _ _ _ p p0 n' d). exact (m, leither _ _ m0).
+  destruct pf. cbv in p. cbv in p0. destruct (runProtoMultiStep' _ _ _ _ p p0 n' d0). exact (m, reither _ _ m0).
+  destruct b.
+    destruct pf. cbv in p. cbv in p0. destruct (runProtoMultiStep' _ _ _ _ p p0 n' d). exact (leither _ _  m, m0).
+    destruct pf. cbv in p. cbv in p0. destruct (runProtoMultiStep' _ _ _ _ p p0 n' d0). exact (reither _ _ m, m0).
+    destruct pf. cbv in p. cbv in p0. assert (Dual p p0). reflexivity. destruct (runProtoMultiStep' _ _ _ _ p p0 n' H). exact (m2, m1). Defined.
 
-Definition incPayload (m:message Basic) : (message Basic) :=
-  match m with
-  | basic n => basic (n + 1)
-  | _ => basic 0                 
-  end.
-  
-Definition proto4 :=
-  x <- receive;
-  send (incPayload x);
-  ReturnC x.
-Check proto4.
-
-Definition proto5 :=
-  send (basic 42);
-  x <- receive;
-  ReturnC (t:=Basic) x.
-Check proto5.
-
-Example dual45 : Dual proto4 proto5. unfold Dual. simpl. auto. Defined.
-
-Eval compute in runProto proto4 proto5 dual45.
-
-Definition proto6 (b:bool) :=
-  choice b EpsC
-         proto5. Check proto6.
-
-Definition proto7 :=
-  offer EpsC
-        proto4. Check proto7.
-
-Example dual67 : forall b, Dual (proto6 b) proto7. unfold Dual. simpl. auto. Defined.
-
-Eval compute in (runProto (proto6 false) proto7 (dual67 false)).
-Eval compute in (runProto (proto6 true) proto7 (dual67 true)).
-
-Example notDual35 : ~ (Dual proto3  proto5). auto. Defined.
-Eval compute in (runProto proto5 proto3).
-
-
-
-Definition aPub := (public 1).
-Definition bPub := (public 2).
-Definition aPubBad := (public 3).
-Definition bPubBad := (public 4).
-Definition aPri := (private 1).
-Definition bPri := (private 2).
-Definition aPriBad := (private 5).
-Definition bPriBad := (private 6).
-
-Definition aNonce := (basic 1).
-Definition bNonce := (basic 2).
-                    
-
-Definition Needham_A (myPri theirPub:keyType) :=
-  send (encrypt aNonce theirPub);
-  x <- receive; (* x : Encrypt (Pair Basic Basic) *) 
-  let y := decryptM x myPri in (* y : Pair Basic Basic *) 
-  let y' := (pairSnd (t1:=Basic) (t2:=Basic) y) in 
-  send (encrypt y' theirPub);
-  ReturnC (t:= Pair Basic Basic) y. Check Needham_A.
-
-Definition Needham_B (myPri theirPub:keyType) :=
-  x <- receive; (* x : Encrypt Basic *)
-  let y := decryptM x myPri in (* y : Basic *)
-  send (encrypt (pair y bNonce) theirPub);
-  z <- receive; (* z : Encrypt Basic *)
-  let z' := decryptM z myPri in    (* z' : Basic *)
-  ReturnC (t:= Pair Basic (Basic)) (pair y z'). Check Needham_B.
-
-
-
-Example DualNeedham {a b c d:keyType} : Dual (Needham_A a b) (Needham_B c d).
-Proof. unfold Dual; simpl. repeat( split;trivial). Defined.
-
-Definition Needham_A_good := (Needham_A aPri bPub).
-Definition Needham_B_good := (Needham_B bPri aPub).
-
-Eval compute in runProto Needham_A_good Needham_B_good DualNeedham.
-
-Definition Needham_A_badAuth := (Needham_A aPriBad bPub).
-Definition Needham_A_badEncrypt := (Needham_A aPri bPubBad).
-Definition Needham_B_badAuth := (Needham_B bPriBad aPub).
-Definition Needham_B_badEncrypt := (Needham_B bPri aPubBad).
-
-(* A is good, B is an intruder.
-   A returns (bad, basic 2).  The bad propogates from the fact that B is
-     unable to decrypt A's first sent message(A's nonce), and hence is 
-     unable to send it back to A.
-   B returns (bad, bad).  The first bad is because B cannot decrypt A's
-     first message.  The second bad is because B cannot decrypt A's second
-     sent message (A sending back the nonce it received from B). *)
-Eval compute in runProto Needham_A_good Needham_B_badAuth DualNeedham.
-
-(* Are the badEncrypt cases worth demonstrating??
-   i.e: Do we care about results when encrypting with the wrong pub key? *)
-Eval compute in runProto Needham_A_good Needham_B_badEncrypt DualNeedham.
-
-Eval compute in runProto Needham_A_badAuth Needham_B_good DualNeedham. 
-Eval compute in runProto Needham_A_badEncrypt Needham_B_good DualNeedham.
-
-Eval compute in runProto Needham_A_badAuth Needham_B_badAuth DualNeedham.
-Eval compute in runProto Needham_A_badAuth Needham_B_badEncrypt DualNeedham.
-
-Eval compute in runProto Needham_A_badEncrypt Needham_B_badAuth DualNeedham.
-Eval compute in runProto Needham_A_badEncrypt Needham_B_badEncrypt DualNeedham.
-
-Definition protoAuth1 (theirPub:keyType) :=
-  let m1 := encrypt (basic 1) theirPub in
-  send m1;
-  x <- receive;
-  ReturnC (t:=Basic) x. Check protoAuth1.
-
-Definition protoAuth2 (myPri:keyType) :=
-  x <- receive;
-  let m1 := decryptM x myPri in
-  send m1;
-    ReturnC (t:=Basic) m1. Check protoAuth2.
-
-Example dualProtoAuth12 {k k':keyType} : Dual (protoAuth1 k) (protoAuth2 k').
-Proof. unfold Dual; simpl. repeat( split;trivial). Defined.
-
-Eval compute in runProto (protoAuth1 (public 2))
-                         (protoAuth2 (private 2))
-                         dualProtoAuth12.
-Eval compute in runProto' (protoAuth1 (public 2))
-                         (protoAuth2 (private 2))
-                         dualProtoAuth12.
-
-Example badAuth : forall k k',
-    (k <> inverse k') ->
-    (runProto' (protoAuth1 k) (protoAuth2 k') dualProtoAuth12)
-    = bad Basic.
-Proof.
-  intros. cbv. Abort.
-
-Example uniqueAuth : forall k k',
-    (runProto' (protoAuth1 k) (protoAuth2 k') dualProtoAuth12)
-      = (basic 1)
-    -> (k = (inverse k')).
-Proof.
-  intros. destruct (is_inverse k k').
-  assumption. cbv in H. Abort.
-  
-       
-End session.
+Definition runProtoMultiStep {t t':protoType} {T T':type} (p1:protoExp T t) (p2:protoExp T' t') : (Dual p1 p2) -> (message T * message T') :=
+  fun pf =>
+  runProtoMultiStep' p1 p2 (max (protoExpLength p1) (protoExpLength p2)) pf.
+                      
+(*End session.*)
